Weidenbach_Book/IsaSAT/IsaSAT_LLVM.thy
@@ -330,12 +330,16 @@ sepref_def print_gc_impl
   unfolding print_gcs_def
   by sepref
 
-definition IsaSAT_bounded_heur_wrapper :: \<open>nat \<Rightarrow> nat \<Rightarrow> nat \<Rightarrow> 64 word \<Rightarrow> 64 word \<Rightarrow> nat \<Rightarrow> _ \<Rightarrow> (nat) nres\<close>where
-  \<open>IsaSAT_bounded_heur_wrapper red res unbdd mini res1 res2 C = do {
-      let opts = IsaOptions (res \<noteq> 0) (res \<noteq> 0)
-         (unbdd \<noteq> 0) mini res1 res2;
+abbreviation (input) C_bool_to_bool :: \<open>8 word \<Rightarrow> bool\<close> where
+  \<open>C_bool_to_bool g \<equiv> g \<noteq> 0\<close>
+
+definition IsaSAT_bounded_heur_wrapper :: \<open>8 word \<Rightarrow> 8 word \<Rightarrow> 8 word \<Rightarrow> 64 word \<Rightarrow> 64 word \<Rightarrow> nat \<Rightarrow> 8 word \<Rightarrow> _ \<Rightarrow> (nat) nres\<close>where
+  \<open>IsaSAT_bounded_heur_wrapper red res unbdd mini res1 res2 target_option C = do {
+      let opts = IsaOptions (C_bool_to_bool red) (C_bool_to_bool res)
+         (C_bool_to_bool unbdd) mini res1 res2
+         (if target_option = 2 then 2 else if target_option = 0 then 0 else 1);
       (b, (b', (_, propa, confl, dec, res, lres, uset, gcs, d))) \<leftarrow> IsaSAT_bounded_heur (opts) C;
-      let _ = print_propa propa; 
+      let _ = print_propa propa;
       let _ = print_confl confl;
       let _ = print_dec dec;
       let _ = print_res res;
@@ -351,10 +355,14 @@ text \<open>
   statistics.
 \<close>
 sepref_register IsaSAT_bounded_heur default_opts
+
+abbreviation bool_C_assn where
+   \<open>bool_C_assn \<equiv> (word_assn' (TYPE(8)))\<close>
+
 sepref_def IsaSAT_code_wrapped
-  is \<open>uncurry6 IsaSAT_bounded_heur_wrapper\<close>
-  :: \<open>snat64_assn\<^sup>k *\<^sub>a snat64_assn\<^sup>k *\<^sub>a snat64_assn\<^sup>k *\<^sub>a word64_assn\<^sup>k *\<^sub>a word64_assn\<^sup>k *\<^sub>a
-      (snat_assn' (TYPE(64)))\<^sup>k *\<^sub>a (clauses_ll_assn)\<^sup>k \<rightarrow>\<^sub>a sint64_nat_assn\<close>
+  is \<open>uncurry7 IsaSAT_bounded_heur_wrapper\<close>
+  :: \<open>bool_C_assn\<^sup>k *\<^sub>a bool_C_assn\<^sup>k *\<^sub>a bool_C_assn\<^sup>k *\<^sub>a word64_assn\<^sup>k *\<^sub>a word64_assn\<^sup>k *\<^sub>a
+      (snat_assn' (TYPE(64)))\<^sup>k *\<^sub>a bool_C_assn\<^sup>k *\<^sub>a (clauses_ll_assn)\<^sup>k \<rightarrow>\<^sub>a sint64_nat_assn\<close>
   supply [[goals_limit=1]] if_splits[split]
   unfolding IsaSAT_bounded_heur_wrapper_def
   apply (annot_snat_const \<open>TYPE(64)\<close>)
@@ -408,9 +416,10 @@ begin
     IsaSAT_code
     count_decided_pol_impl is \<open>uint32_t count_decided_st_heur_pol_fast(TRAIL)\<close>
     arena_lit_impl is \<open>uint32_t arena_lit_impl(ARENA, int64_t)\<close>
-    IsaSAT_code_wrapped is \<open>int64_t IsaSAT_wrapped(int64_t, int64_t, int64_t,
-        int64_t, int64_t, int64_t, CLAUSES)\<close>
+    IsaSAT_code_wrapped is \<open>int64_t IsaSAT_wrapped(CBOOL, CBOOL, CBOOL,
+        int64_t, int64_t, int64_t, CBOOL, CLAUSES)\<close>
   defines \<open>
+     typedef int8_t CBOOL;
      typedef struct {int64_t size; struct {int64_t used; uint32_t *clause;};} CLAUSE;
      typedef struct {int64_t num_clauses; CLAUSE *clauses;} CLAUSES;
 
